Everything close to compile
but I get a circular dependency error

Other things to look at:
- safety checker port is ugly
- signature in stack_alloc.mli ugly too (but not sure we can do better)
- primP in 3 versions...
- is prim_string in asmOp in sopn.v a good idea?
- cleanings about pp_opn

compiler/src/help.ml
@@ -1,6 +1,6 @@
 open Pretyping
 
-let show_intrinsics fmt =
+let show_intrinsics asmOp fmt =
   let index =
     function
     | PrimM _ -> 0
@@ -20,7 +20,7 @@ let show_intrinsics fmt =
   List.iter (fun (n, i) ->
       let j = index i in
       intrinsics.(j) <- n :: intrinsics.(j))
-    prim_string;
+    (prim_string asmOp);
   Array.iter2 (fun h m ->
       Format.fprintf fmt "Intrinsics accepting %s:@." h;
       m |>
@@ -29,5 +29,5 @@ let show_intrinsics fmt =
       Format.fprintf fmt "@."
     ) headers intrinsics
 
-let show_intrinsics () =
-  show_intrinsics Format.std_formatter
+let show_intrinsics asmOp () =
+  show_intrinsics asmOp Format.std_formatter
