compiler/src/toEC.mli
@@ -1,6 +1,11 @@
 val ty_expr : Prog.expr -> Prog.ty
 val ty_lval : Prog.lval -> Prog.ty
-val extract : Format.formatter ->
-        Utils.model -> ('a, 'asm) Prog.prog -> string list -> unit
+val extract :
+  ('reg, 'xreg, 'rflag, 'cond, 'asm_op, 'extra_op) Arch_extra.extended_op Sopn.asmOp ->
+  (Format.formatter ->
+    ('reg, 'xreg, 'rflag, 'cond, 'asm_op, 'extra_op) Arch_extra.extended_op Sopn.sopn -> unit) ->
+  Format.formatter ->
+  Utils.model -> ('info, ('reg, 'xreg, 'rflag, 'cond, 'asm_op, 'extra_op) Arch_extra.extended_op) Prog.prog ->
+  string list -> unit
 
 val init_use : ('info, 'asm) Prog.func list -> Prog.Sf.t * Prog.Sf.t
